dataplane/Common_Operators/Increment_Op.thy
@@ -4,7 +4,7 @@ imports
   "../Timely/Builder_Op"
 begin
 
-definition \<open>increment_op_logic ip op inc = (\<lambda>os. 
+definition \<open>incr_op_logic ip op inc = (\<lambda>os. 
     if ocaps os op = [] then {||} else
     {|
       let result = map (\<lambda>(d, t). (d, t + inc)) (input os ip);
@@ -12,98 +12,98 @@ definition \<open>increment_op_logic ip op inc = (\<lambda>os.
           os'' = drop_caps os' (map (\<lambda>t. Cap t op) (ocaps os' op))
       in os''\<lparr>input := (input os)(op := [])\<rparr>|})\<close>
 
-definition \<open>increment_op ip op inc os = builder_op False {|ip|} {|op|} os (increment_op_logic ip op inc)\<close>
+definition \<open>incr_op ip op inc os = builder_op False {|ip|} {|op|} os (incr_op_logic ip op inc)\<close>
 
-lemma increment_op_logic_front_initia:
-  "os' |\<in>| increment_op_logic ip op inc os \<Longrightarrow> front os' = front os"
-  "os' |\<in>| increment_op_logic ip op inc os \<Longrightarrow> initia os' = initia os"
-  unfolding increment_op_logic_def
+lemma incr_op_logic_front_initia:
+  "os' |\<in>| incr_op_logic ip op inc os \<Longrightarrow> front os' = front os"
+  "os' |\<in>| incr_op_logic ip op inc os \<Longrightarrow> initia os' = initia os"
+  unfolding incr_op_logic_def
   by (auto simp add: Let_def split: if_splits simp flip: cin.rep_eq)
 
-lemma nop_leaf_increment_op:
-  "nop_leaf None (increment_op ip op inc os)"
-  unfolding increment_op_def
+lemma nop_leaf_incr_op:
+  "nop_leaf None (incr_op ip op inc os)"
+  unfolding incr_op_def
   by (rule nop_leaf_builder_op) simp
 
-section \<open>Inputs of increment_op\<close>
+section \<open>Inputs of incr_op\<close>
 
-lemma inputs_increment_op:
-  assumes \<open>sub_op (Read p f) (increment_op ip op inc os) n\<close>
+lemma inputs_incr_op:
+  assumes \<open>sub_op (Read p f) (incr_op ip op inc os) n\<close>
   shows \<open>p = Some ip\<close>
   using assms
-proof (induct p \<open>increment_op ip op inc os\<close> arbitrary: os rule: sub_op_Read_induct)
+proof (induct p \<open>incr_op ip op inc os\<close> arbitrary: os rule: sub_op_Read_induct)
   case (Read1 f p)
   then show ?case
-    unfolding increment_op_def
+    unfolding incr_op_def
     by (subst (asm) builder_op.code) (auto split: if_splits option.splits list.splits sum.splits)
 next
   case (Read2 p p' f x d g)
   then show ?case
-    unfolding increment_op_def
+    unfolding incr_op_def
     by (subst (asm) builder_op.code) (auto split: if_splits option.splits list.splits sum.splits)
 next
   case (Write p p' op' x d g)
   then show ?case
-    unfolding increment_op_def
+    unfolding incr_op_def
     by (subst (asm) builder_op.code) (auto split: if_splits option.splits list.splits sum.splits)
 next
   case (Silent p op' d)
   then show ?case
-    unfolding increment_op_def
+    unfolding incr_op_def
     by (subst (asm) builder_op.code) (auto split: if_splits option.splits list.splits sum.splits)
 next
   case (Choice p choices d g)
   then show ?case
-    unfolding increment_op_def
+    unfolding incr_op_def
     apply -
     apply (subst (asm) (2) builder_op.code)
     apply (auto 0 0 simp add: obtain_progress_def
-        simp del: increment_op_logic_front_initia
+        simp del: incr_op_logic_front_initia
         operator_state_front_initia_upd_collapse
         split: if_splits list.splits sum.splits prod.splits)
     apply (meson Suc_lessD lessI)+
     done
 qed
 
-lemma inputs_increment_op_le:
-  \<open>inputs (increment_op ip op inc os) \<subseteq> {Some ip}\<close>
-  by (auto dest!: inputs_sub_op_Read inputs_increment_op)
+lemma inputs_incr_op_le:
+  \<open>inputs (incr_op ip op inc os) \<subseteq> {Some ip}\<close>
+  by (auto dest!: inputs_sub_op_Read inputs_incr_op)
 
 
-lemma inputs_increment_op_le_alt[dest!]:
-  \<open>p \<in> inputs (increment_op ip op inc os) \<Longrightarrow> p = Some ip\<close>
-  using set_mp[OF inputs_increment_op_le] by blast
+lemma inputs_incr_op_le_alt[dest!]:
+  \<open>p \<in> inputs (incr_op ip op inc os) \<Longrightarrow> p = Some ip\<close>
+  using set_mp[OF inputs_incr_op_le] by blast
 
 
-section \<open>Introduction rules for increment_op steps\<close>
+section \<open>Introduction rules for incr_op steps\<close>
 
-lemma step_increment_op_Write_None[intro]:
+lemma step_incr_op_Write_None[intro]:
   assumes \<open>io = Out None (Inl (Inl st))\<close>
     and \<open>(os', st) = obtain_progress os\<close>
-    and \<open>op' = increment_op ip op inc os'\<close>
-  shows \<open>step io (increment_op ip op inc os) op'\<close>
-  using assms unfolding increment_op_def by auto
+    and \<open>op' = incr_op ip op inc os'\<close>
+  shows \<open>step io (incr_op ip op inc os) op'\<close>
+  using assms unfolding incr_op_def by auto
 
-lemma step_increment_op_Write_None_alt[intro]:
+lemma step_incr_op_Write_None_alt[intro]:
   assumes \<open>io = Out None (Inl (Inl (snd (obtain_progress os))))\<close>
-    and \<open>op' = increment_op ip op inc (fst (obtain_progress os))\<close>
-  shows \<open>step io (increment_op ip op inc os) op'\<close>
-  by (rule step_increment_op_Write_None[OF assms(1) _ assms(2)]) (rule prod.collapse)
+    and \<open>op' = incr_op ip op inc (fst (obtain_progress os))\<close>
+  shows \<open>step io (incr_op ip op inc os) op'\<close>
+  by (rule step_incr_op_Write_None[OF assms(1) _ assms(2)]) (rule prod.collapse)
 
-lemma steps_increment_op_Write_Some[intro]:
+lemma steps_incr_op_Write_Some[intro]:
   assumes \<open>outpu os op = xs @ ys\<close>
-    and \<open>op' = increment_op ip op inc (os\<lparr>outpu := (outpu os)(op := ys)\<rparr>)\<close>
+    and \<open>op' = incr_op ip op inc (os\<lparr>outpu := (outpu os)(op := ys)\<rparr>)\<close>
     and \<open>zs = map (\<lambda>x. Out (Some op) (Inr x)) xs\<close>
-  shows \<open>steps zs (increment_op ip op inc os) op'\<close>
-  using assms unfolding increment_op_def by auto
+  shows \<open>steps zs (incr_op ip op inc os) op'\<close>
+  using assms unfolding incr_op_def by auto
 
-lemma steps_increment_op_Read_Some[intro]:
-  assumes \<open>op' = increment_op ip op inc (fold (\<lambda>(d, t) os. consumes os ip t d) xs os)\<close>
+lemma steps_incr_op_Read_Some[intro]:
+  assumes \<open>op' = incr_op ip op inc (fold (\<lambda>(d, t) os. consumes os ip t d) xs os)\<close>
     and \<open>ys = map (\<lambda>x. Inp (Some ip) (Inr x)) xs\<close>
-  shows \<open>steps ys (increment_op ip op inc os) op'\<close>
-  using assms unfolding increment_op_def by auto
+  shows \<open>steps ys (incr_op ip op inc os) op'\<close>
+  using assms unfolding incr_op_def by auto
 
-lemma step_increment_op_Silent[intro]:
+lemma step_incr_op_Silent[intro]:
   assumes \<open>ocaps os op \<noteq> []\<close>
     and \<open>result = map (\<lambda>(d, t). (d, t + inc)) (input os ip)\<close>
     and \<open>os_produced = produces os (map (\<lambda>(d, t). (d, Cap t op)) result)\<close>
@@ -111,15 +111,15 @@ lemma step_increment_op_Silent[intro]:
     and \<open>os_dropped = drop_caps os_produced caps\<close>
     and \<open>os_next = os_dropped\<lparr>input := (input os_dropped)(op := [])\<rparr>\<close>
     and \<open>initia os\<close>
-    and \<open>op' = increment_op ip op inc os_next\<close>
-  shows \<open>step Tau (increment_op ip op inc os) op'\<close>
-  unfolding assms(8) increment_op_def
+    and \<open>op' = incr_op ip op inc os_next\<close>
+  shows \<open>step Tau (incr_op ip op inc os) op'\<close>
+  unfolding assms(8) incr_op_def
   apply (rule step_builder_op_Silent)
      apply (rule refl)
     apply (rule assms(7))
-   apply (unfold increment_op_logic_def)
+   apply (unfold incr_op_logic_def)
    apply (simp add: assms(1-6))
-  apply (simp add: assms(2-6) increment_op_logic_front_initia
+  apply (simp add: assms(2-6) incr_op_logic_front_initia
       operator_state_front_initia_upd_collapse)
   done
 
