dataplane/Common_Operators/Increment_Op_Correctness.thy
@@ -14,22 +14,22 @@ lemma append_append_lshift:
   \<open>(xs @ ys @ zs) @@- lxs = xs @@- (ys @ zs) @@- lxs\<close>
   using lappend_assoc lappend_llist_of lappend_llist_of_llist_of by metis
 
-lemma ooo_input_op_increment_op_source_op:
+lemma ooo_input_op_incr_op_source_op:
   defines \<open>invariant f inc os1 buf os2 \<equiv> initia os1 \<and> en1 os1 = f
   \<and> timely_input_stream (es os1 1) (mset (ocaps os1 1)) \<and> (\<forall>x \<in> set (buf (Inr (1, 1))). is_Inr x)
   \<and> initia os2 \<and> intsum os2 1 1 = [inc] \<and> ocaps os2 1 = map (\<lambda>(_, t). t + inc) (input os2 1)\<close>
     and \<open>my_ooo_input_op os \<equiv> map_op
   (case_option (Inl (0 :: 2)) (\<lambda>(p :: 1). Inr (0 :: 2, 1))) (case_option (Inl (0 :: 2)) (\<lambda>(p :: 1). Inr (0 :: 2, 1)))
   (ooo_input_op {|1 :: 1|} os)\<close>
-    and \<open>my_increment_op inc os' \<equiv> map_op
+    and \<open>my_incr_op inc os' \<equiv> map_op
   (case_option (Inl (1 :: 2)) (\<lambda>(p :: 1). Inr (1 :: 2, 1))) (case_option (Inl (1 :: 2)) (\<lambda>(p :: 1). Inr (1 :: 2, 1)))
-  (increment_op (1 :: 1) (1 :: 1) inc os')\<close>
+  (incr_op (1 :: 1) (1 :: 1) inc os')\<close>
     and \<open>my_source_op f inc os1 buf os2 \<equiv> map_op (\<lambda>(p :: 1). (1, 1)) (\<lambda>(p :: 1). (1, 1))
     (source_op ((\<lambda>(p :: 1). outpu os2 1 @@- lmap (\<lambda>(d, t). (d, t + inc))
       ((input os2 1 @ map projr (buf (Inr (1, 1))) @ outpu os1 1) @@- lmap (\<lambda>x. case x of Data t d \<Rightarrow> (f d, t)) (lfilter is_Data (es os1 1))))))\<close>
   assumes \<open>invariant f inc os1 buf os2\<close>
   shows \<open>dataflow_op sg (map_op (case_sum id id) (case_sum id id)
-  (comp_op [Inr (0 :: 2, 1 :: 1) \<mapsto> Inr (1 :: 2, 1 :: 1)] buf (my_ooo_input_op os1) (my_increment_op inc os2)))
+  (comp_op [Inr (0 :: 2, 1 :: 1) \<mapsto> Inr (1 :: 2, 1 :: 1)] buf (my_ooo_input_op os1) (my_incr_op inc os2)))
   \<approx> my_source_op f inc os1 buf os2\<close>
   using assms(5)
 proof (coinduction arbitrary: sg os1 buf os2 rule: wbisim_coinduct_upto'')
@@ -43,8 +43,8 @@ proof (coinduction arbitrary: sg os1 buf os2 rule: wbisim_coinduct_upto'')
     proof -
       have "\<exists>op2'. wstep (Out (1, 1) (d, t)) (my_source_op f inc os1 buf os2) op2'
   \<and> wbisim_cong R (dataflow_op sg (map_op (case_sum id id) (case_sum id id) (comp_op [Inr (0, 1) \<mapsto> Inr (1, 1)] buf
-    (my_ooo_input_op os1) (my_increment_op inc (os2\<lparr>outpu := (outpu os2)(1 := xs)\<rparr>))))) op2'"
-        (is \<open>\<exists>_. _ \<and> wbisim_cong _ (dataflow_op _ (map_op _ _ (comp_op _ _ _ (my_increment_op _ ?os2')))) _\<close>)
+    (my_ooo_input_op os1) (my_incr_op inc (os2\<lparr>outpu := (outpu os2)(1 := xs)\<rparr>))))) op2'"
+        (is \<open>\<exists>_. _ \<and> wbisim_cong _ (dataflow_op _ (map_op _ _ (comp_op _ _ _ (my_incr_op _ ?os2')))) _\<close>)
         if "invariant f inc os1 buf os2"
           and "outpu os2 1 = (d, t) # xs"
         for d :: 'b
@@ -63,7 +63,7 @@ proof (coinduction arbitrary: sg os1 buf os2 rule: wbisim_coinduct_upto'')
       qed
       moreover have "\<exists>op2'. (step Tau)\<^sup>*\<^sup>* (my_source_op f inc os1 buf os2) op2'
   \<and> wbisim_cong R (dataflow_op sg (map_op (case_sum id id) (case_sum id id) (comp_op [Inr (0, 1) \<mapsto> Inr (1, 1)] (BENQ (Inr (1, 1)) (Inr (d, t)) buf)
-    (my_ooo_input_op (os1\<lparr>outpu := (outpu os1)(1 := xs)\<rparr>)) (my_increment_op inc os2)))) op2'"
+    (my_ooo_input_op (os1\<lparr>outpu := (outpu os1)(1 := xs)\<rparr>)) (my_incr_op inc os2)))) op2'"
         (is \<open>\<exists>_. _ \<and> wbisim_cong _ (dataflow_op _ (map_op _ _ (comp_op _ ?buf' (my_ooo_input_op ?os1') _))) _\<close>)
         if "invariant f inc os1 buf os2"
           and "outpu os1 1 = (d, t) # xs"
@@ -85,8 +85,8 @@ proof (coinduction arbitrary: sg os1 buf os2 rule: wbisim_coinduct_upto'')
         by (metis (no_types, opaque_lifting))
       moreover have "\<exists>op2'. (step Tau)\<^sup>*\<^sup>* (my_source_op f inc os1 buf os2) op2'
   \<and> wbisim_cong R (dataflow_op sg (map_op (case_sum id id) (case_sum id id) (comp_op [Inr (0, 1) \<mapsto> Inr (1, 1)] (BTL (Inr (1, 1)) buf)
-    (my_ooo_input_op os1) (my_increment_op inc (consumes os2 1 t d))))) op2'"
-        (is \<open>\<exists>_. _ \<and> wbisim_cong _ (dataflow_op _ (map_op _ _ (comp_op _ ?buf' _ (my_increment_op _ ?os2')))) _\<close>)
+    (my_ooo_input_op os1) (my_incr_op inc (consumes os2 1 t d))))) op2'"
+        (is \<open>\<exists>_. _ \<and> wbisim_cong _ (dataflow_op _ (map_op _ _ (comp_op _ ?buf' _ (my_incr_op _ ?os2')))) _\<close>)
         if "invariant f inc os1 buf os2"
           and "buf (Inr (1, 1)) \<noteq> []"
           and "Inr (d, t) = BHD (Inr (1, 1)) buf"
@@ -105,7 +105,7 @@ proof (coinduction arbitrary: sg os1 buf os2 rule: wbisim_coinduct_upto'')
       qed
       moreover have "\<exists>op2'. (step Tau)\<^sup>*\<^sup>* (my_source_op f inc os1 buf os2) op2'
   \<and> wbisim_cong R (dataflow_op sg (map_op (case_sum id id) (case_sum id id) (comp_op [Inr (0, 1) \<mapsto> Inr (1, 1)] buf
-  (my_ooo_input_op os1') (my_increment_op inc os2)))) op2'"
+  (my_ooo_input_op os1') (my_incr_op inc os2)))) op2'"
         if "invariant f inc os1 buf os2"
           and "os1' |\<in>| ooo_input_op_logic {|1|} os1"
         for os1' :: "(1, 'b, 'a, 'c, 'd) input_state_scheme"
@@ -121,23 +121,23 @@ proof (coinduction arbitrary: sg os1 buf os2 rule: wbisim_coinduct_upto'')
       qed
       moreover have "\<exists>op2'. (step Tau)\<^sup>*\<^sup>* (my_source_op f inc os1 buf os2) op2'
   \<and> wbisim_cong R (dataflow_op sg (map_op (case_sum id id) (case_sum id id) (comp_op [Inr (0, 1) \<mapsto> Inr (1, 1)] buf
-  (my_ooo_input_op os1) (my_increment_op inc os2')))) op2'"
+  (my_ooo_input_op os1) (my_incr_op inc os2')))) op2'"
         if "invariant f inc os1 buf os2"
-          and "os2' |\<in>| increment_op_logic 1 1 inc os2"
+          and "os2' |\<in>| incr_op_logic 1 1 inc os2"
         for os2' :: "(1, 'b, 'c, 'e) operator_state_scheme"
       proof -
         have outpu_os2': \<open>outpu os2' 1 = outpu os2 1 @ map (\<lambda>(d, t). (d, t + inc)) (input os2 1)\<close>
-          using that(2) unfolding trace_simp increment_op_logic_def drop_caps_def release_caps_def produces_def by (simp split: prod.splits if_splits)
-        have input_os2': \<open>input os2' 1 = []\<close> using that(2) unfolding increment_op_logic_def by (simp split: prod.splits if_splits)
+          using that(2) unfolding trace_simp incr_op_logic_def drop_caps_def release_caps_def produces_def by (simp split: prod.splits if_splits)
+        have input_os2': \<open>input os2' 1 = []\<close> using that(2) unfolding incr_op_logic_def by (simp split: prod.splits if_splits)
         have \<open>my_source_op f inc os1 buf os2 = my_source_op f inc os1 buf os2'\<close>
           using outpu_os2' input_os2' unfolding my_source_op_def by (simp add: lshift_append_lshift)
         moreover have \<open>invariant f inc os1 buf os2'\<close> using that unfolding invariant_def
-            increment_op_logic_def release_caps_def drop_caps_def produces_def enum_num1_def by (simp add: comp_def split: prod.splits if_splits)
+            incr_op_logic_def release_caps_def drop_caps_def produces_def enum_num1_def by (simp add: comp_def split: prod.splits if_splits)
         ultimately show ?thesis unfolding R_def by blast
       qed
       moreover have "\<exists>op2'. (step Tau)\<^sup>*\<^sup>* (my_source_op f inc os1 buf os2) op2'
   \<and> wbisim_cong R (dataflow_op (sg\<lparr>pt_tr := change_multiplicities (summ sg) (extract_progress 1 (nxt sg) st) (pt_tr sg)\<rparr>) (map_op (case_sum id id) (case_sum id id) (comp_op [Inr (0, 1) \<mapsto> Inr (1, 1)] buf
-    (my_ooo_input_op os1) (my_increment_op inc os2')))) op2'"
+    (my_ooo_input_op os1) (my_incr_op inc os2')))) op2'"
         if "invariant f inc os1 buf os2"
           and "(os2', st) = obtain_progress os2"
         for st :: "(1, 'c) shared_state"
@@ -145,7 +145,7 @@ proof (coinduction arbitrary: sg os1 buf os2 rule: wbisim_coinduct_upto'')
         using that unfolding R_def invariant_def my_source_op_def obtain_progress_def by (fastforce intro!: wbc_base)
       moreover have "\<exists>op2'. (step Tau)\<^sup>*\<^sup>* (my_source_op f inc os1 buf os2) op2'
   \<and> wbisim_cong R (dataflow_op (sg\<lparr>pt_tr := change_multiplicities (summ sg) (extract_progress 0 (nxt sg) st) (pt_tr sg)\<rparr>) (map_op (case_sum id id) (case_sum id id) (comp_op [Inr (0, 1) \<mapsto> Inr (1, 1)] buf
-  (my_ooo_input_op os1') (my_increment_op inc os2)))) op2'"
+  (my_ooo_input_op os1') (my_incr_op inc os2)))) op2'"
         if "invariant f inc os1 buf os2"
           and "(os1', st) = obtain_progress os1"
         for st :: "(1, 'c) shared_state"
@@ -153,10 +153,10 @@ proof (coinduction arbitrary: sg os1 buf os2 rule: wbisim_coinduct_upto'')
         using that unfolding R_def invariant_def my_source_op_def obtain_progress_def by (fastforce intro!: wbc_base)
       ultimately show ?thesis unfolding R_def[symmetric]
         by (sim_cases sim: SIM1
-            defs: my_ooo_input_op_def ooo_input_op_def my_increment_op_def increment_op_def
+            defs: my_ooo_input_op_def ooo_input_op_def my_incr_op_def incr_op_def
             elims: step_dataflow_op_elim step_map_op_elim step_comp_op_elim step_builder_op_elim
             intros: invariant_initia
-            simps: ooo_input_op_logic_front_initia increment_op_logic_front_initia
+            simps: ooo_input_op_logic_front_initia incr_op_logic_front_initia
             operator_state_front_initia_upd_collapse)
     qed
   qed
@@ -166,7 +166,7 @@ next
   proof -
     define R where \<open>R = ?R\<close>
     have "\<exists>op2'. wstep (Out (1, 1) (d, t)) (dataflow_op sg (map_op (case_sum id id) (case_sum id id)
-    (comp_op [Inr (0, 1) \<mapsto> Inr (1, 1)] buf (my_ooo_input_op os1) (my_increment_op inc os2)))) op2'
+    (comp_op [Inr (0, 1) \<mapsto> Inr (1, 1)] buf (my_ooo_input_op os1) (my_incr_op inc os2)))) op2'
   \<and> wbisim_cong R op2' (map_op (\<lambda>(p :: 1). (1, 1)) (\<lambda>p. (1, 1)) (source_op ((\<lambda>(p :: 1). LCons (d, t) lxs)(1 := lxs))))"
       if inv: "invariant f inc os1 buf os2"
         and source_llist: "outpu os2 1 @@- lmap (\<lambda>(d, t). (d, t + inc)) ((input os2 1 @ map projr (buf (Inr (1, 1))) @ outpu os1 1)
@@ -215,9 +215,9 @@ next
               unfolding invariant_def timely_input_stream_def by simp
             hence step_Taus: \<open>(step Tau)\<^sup>*\<^sup>*
   (dataflow_op sg (map_op (case_sum id id) (case_sum id id) (comp_op [Inr (0, 1) \<mapsto> Inr (1, 1)] buf
-    (my_ooo_input_op os1) (my_increment_op inc os2))))
+    (my_ooo_input_op os1) (my_incr_op inc os2))))
   (dataflow_op sg (map_op (case_sum id id) (case_sum id id) (comp_op [Inr (0, 1) \<mapsto> Inr (1, 1)] buf
-    (my_ooo_input_op ?os1_2) (my_increment_op inc os2))))\<close> unfolding my_ooo_input_op_def by fast
+    (my_ooo_input_op ?os1_2) (my_incr_op inc os2))))\<close> unfolding my_ooo_input_op_def by fast
             have initia_os1_2: \<open>initia ?os1_2\<close> using that(1) foldl_ooo_input_os_Drop_Mint(1)[OF set_not_Data]
               unfolding invariant_def produces_def by fastforce
             have outpu_os1_2: \<open>outpu ?os1_2 1 = [(d, t')]\<close>
@@ -232,9 +232,9 @@ next
             let ?os1_3 = \<open>?os1_2\<lparr>outpu := (outpu ?os1_2)(1 := [])\<rparr>\<close>
             have step_Tau_1: \<open>step Tau
   (dataflow_op sg (map_op (case_sum id id) (case_sum id id) (comp_op [Inr (0, 1) \<mapsto> Inr (1, 1)] buf
-    (my_ooo_input_op ?os1_2) (my_increment_op inc os2))))
+    (my_ooo_input_op ?os1_2) (my_incr_op inc os2))))
   (dataflow_op sg (map_op (case_sum id id) (case_sum id id) (comp_op [Inr (0, 1) \<mapsto> Inr (1, 1)] (BENQ (Inr (1, 1)) (Inr (d, t')) buf)
-    (my_ooo_input_op ?os1_3) (my_increment_op inc os2))))\<close> using initia_os1_2 outpu_os1_2
+    (my_ooo_input_op ?os1_3) (my_incr_op inc os2))))\<close> using initia_os1_2 outpu_os1_2
             proof -
               have \<open>step (Out (Some 1) (Inr (d, t')))
   (ooo_input_op {|1 :: 1|} ?os1_2) (ooo_input_op {|1 :: 1|} ?os1_3)\<close>
@@ -243,16 +243,16 @@ next
   (my_ooo_input_op ?os1_2) (my_ooo_input_op ?os1_3)\<close>
                 unfolding my_ooo_input_op_def by (rule step_map_op) simp
               hence \<open>step Tau
-  (comp_op [Inr (0, 1) \<mapsto> Inr (1, 1)] buf (my_ooo_input_op ?os1_2) (my_increment_op inc os2))
+  (comp_op [Inr (0, 1) \<mapsto> Inr (1, 1)] buf (my_ooo_input_op ?os1_2) (my_incr_op inc os2))
   (comp_op [Inr (0, 1) \<mapsto> Inr (1, 1)] (BENQ (Inr (1, 1)) (Inr (d, t')) buf)
-    (my_ooo_input_op ?os1_3) (my_increment_op inc os2))\<close>
+    (my_ooo_input_op ?os1_3) (my_incr_op inc os2))\<close>
                 by (rule step_Tau_comp_op_L_alt) simp
               hence \<open>step Tau
   (map_op (case_sum id id) (case_sum id id)
-    (comp_op [Inr (0, 1) \<mapsto> Inr (1, 1)] buf (my_ooo_input_op ?os1_2) (my_increment_op inc os2)))
+    (comp_op [Inr (0, 1) \<mapsto> Inr (1, 1)] buf (my_ooo_input_op ?os1_2) (my_incr_op inc os2)))
   (map_op (case_sum id id) (case_sum id id)
     (comp_op [Inr (0, 1) \<mapsto> Inr (1, 1)] (BENQ (Inr (1, 1)) (Inr (d, t')) buf)
-      (my_ooo_input_op ?os1_3) (my_increment_op inc os2)))\<close>
+      (my_ooo_input_op ?os1_3) (my_incr_op inc os2)))\<close>
                 by (rule step_map_op) simp
               thus ?thesis
                 by (rule step_Tau_dataflow_op_Tau_intro)
@@ -260,48 +260,48 @@ next
             let ?os2_1 = \<open>consumes os2 1 t' d\<close>
             have step_Tau_2: \<open>step Tau
   (dataflow_op sg (map_op (case_sum id id) (case_sum id id) (comp_op [Inr (0, 1) \<mapsto> Inr (1, 1)] (BENQ (Inr (1, 1)) (Inr (d, t')) buf)
-    (my_ooo_input_op ?os1_3) (my_increment_op inc os2))))
+    (my_ooo_input_op ?os1_3) (my_incr_op inc os2))))
   (dataflow_op sg (map_op (case_sum id id) (case_sum id id) (comp_op [Inr (0, 1) \<mapsto> Inr (1, 1)] buf
-    (my_ooo_input_op ?os1_3) (my_increment_op inc ?os2_1))))\<close> using that(1) buf_Nil
-              unfolding invariant_def my_increment_op_def increment_op_def
+    (my_ooo_input_op ?os1_3) (my_incr_op inc ?os2_1))))\<close> using that(1) buf_Nil
+              unfolding invariant_def my_incr_op_def incr_op_def
               by (auto intro!: step_Tau_dataflow_op_Tau_intro)
-            obtain os2_2 where os2_2: \<open>os2_2 |\<in>| increment_op_logic 1 1 inc ?os2_1\<close>
-              unfolding increment_op_logic_def trace_simp Let_def 
+            obtain os2_2 where os2_2: \<open>os2_2 |\<in>| incr_op_logic 1 1 inc ?os2_1\<close>
+              unfolding incr_op_logic_def trace_simp Let_def 
               using inv invariant_def by force
-            hence initia_os2_2: \<open>initia os2_2\<close> using that(1) unfolding invariant_def increment_op_logic_def
+            hence initia_os2_2: \<open>initia os2_2\<close> using that(1) unfolding invariant_def incr_op_logic_def
                 consumes_def add_caps_def drop_caps_def produces_def by simp
-            have input_os2_2: \<open>input os2_2 1 = []\<close> using os2_2 unfolding increment_op_logic_def by (simp split: prod.splits if_splits)
+            have input_os2_2: \<open>input os2_2 1 = []\<close> using os2_2 unfolding incr_op_logic_def by (simp split: prod.splits if_splits)
             have outpu_os2_2: \<open>outpu os2_2 1 = [(d, t)]\<close> using outpu_os2_Nil input_os2_Nil os2_2 t'_d'(2)
-              unfolding increment_op_logic_def consumes_def add_caps_def drop_caps_def produces_def
+              unfolding incr_op_logic_def consumes_def add_caps_def drop_caps_def produces_def
               by (simp split: prod.splits if_splits)
             have summar_os2_2: \<open>intsum os2_2 1 1 = [inc]\<close> using that(1) os2_2 unfolding invariant_def
-                increment_op_logic_def consumes_def add_caps_def drop_caps_def produces_def by simp
-            have ocaps_os2_2: \<open>ocaps os2_2 1 = []\<close> using os2_2 unfolding increment_op_logic_def
+                incr_op_logic_def consumes_def add_caps_def drop_caps_def produces_def by simp
+            have ocaps_os2_2: \<open>ocaps os2_2 1 = []\<close> using os2_2 unfolding incr_op_logic_def
                 consumes_def add_caps_def drop_caps_def produces_def enum_num1_def by (simp add: comp_def split: prod.splits if_splits)
-            have \<open>step Tau (my_increment_op inc ?os2_1) (my_increment_op inc os2_2)\<close> using that(1)
-                Cons os2_2 unfolding invariant_def my_increment_op_def increment_op_def consumes_def
+            have \<open>step Tau (my_incr_op inc ?os2_1) (my_incr_op inc os2_2)\<close> using that(1)
+                Cons os2_2 unfolding invariant_def my_incr_op_def incr_op_def consumes_def
                 add_caps_def by (auto intro!: step_builder_op_Silent
-                  simp add: increment_op_logic_front_initia
+                  simp add: incr_op_logic_front_initia
                   operator_state_front_initia_upd_collapse)
             hence step_Tau_3: \<open>step Tau
   (dataflow_op sg (map_op (case_sum id id) (case_sum id id) (comp_op [Inr (0, 1) \<mapsto> Inr (1, 1)] buf
-    (my_ooo_input_op ?os1_3) (my_increment_op inc ?os2_1))))
+    (my_ooo_input_op ?os1_3) (my_incr_op inc ?os2_1))))
   (dataflow_op sg (map_op (case_sum id id) (case_sum id id) (comp_op [Inr (0, 1) \<mapsto> Inr (1, 1)] buf
-    (my_ooo_input_op ?os1_3) (my_increment_op inc os2_2))))\<close> by auto
+    (my_ooo_input_op ?os1_3) (my_incr_op inc os2_2))))\<close> by auto
             let ?os2_3 = \<open>os2_2\<lparr>outpu := (outpu os2_2)(1 := [])\<rparr>\<close>
-            have \<open>step (Out (Inr (1, 1)) (Inr (d, t))) (my_increment_op inc os2_2) (my_increment_op inc ?os2_3)\<close>
+            have \<open>step (Out (Inr (1, 1)) (Inr (d, t))) (my_incr_op inc os2_2) (my_incr_op inc ?os2_3)\<close>
               using that outpu_os2_Nil input_os2_Nil Cons t'_d'(2) initia_os2_2 outpu_os2_2
-              unfolding invariant_def my_increment_op_def increment_op_def by auto
+              unfolding invariant_def my_incr_op_def incr_op_def by auto
             hence \<open>step (Out (1, 1) (d, t))
   (dataflow_op sg (map_op (case_sum id id) (case_sum id id) (comp_op [Inr (0, 1) \<mapsto> Inr (1, 1)] buf
-    (my_ooo_input_op ?os1_3) (my_increment_op inc os2_2))))
+    (my_ooo_input_op ?os1_3) (my_incr_op inc os2_2))))
   (dataflow_op sg (map_op (case_sum id id) (case_sum id id) (comp_op [Inr (0, 1) \<mapsto> Inr (1, 1)] buf
-    (my_ooo_input_op ?os1_3) (my_increment_op inc ?os2_3))))\<close> by auto
+    (my_ooo_input_op ?os1_3) (my_incr_op inc ?os2_3))))\<close> by auto
             hence \<open>wstep (Out (1, 1) (d, t))
   (dataflow_op sg (map_op (case_sum id id) (case_sum id id) (comp_op [Inr (0, 1) \<mapsto> Inr (1, 1)] buf
-    (my_ooo_input_op os1) (my_increment_op inc os2))))
+    (my_ooo_input_op os1) (my_incr_op inc os2))))
   (dataflow_op sg (map_op (case_sum id id) (case_sum id id) (comp_op [Inr (0, 1) \<mapsto> Inr (1, 1)] buf
-    (my_ooo_input_op ?os1_3) (my_increment_op inc ?os2_3))))\<close> using step_Taus step_Tau_1 step_Tau_2
+    (my_ooo_input_op ?os1_3) (my_incr_op inc ?os2_3))))\<close> using step_Taus step_Tau_1 step_Tau_2
               step_Tau_3 step_tau_step_io_wstep wstep_trans'(1) wstep_trans_tau_1 by meson
             moreover have \<open>map_op (\<lambda>(p :: 1). (1, 1)) (\<lambda>(p :: 1). (1, 1)) (source_op ((\<lambda>(p :: 1). LCons (d, t) lxs)(1 := lxs)))
   = my_source_op f inc ?os1_3 buf ?os2_3\<close> using that(2) outpu_os2_Nil input_os2_Nil buf_Nil
@@ -318,56 +318,56 @@ next
             let ?os1' = \<open>os1\<lparr>outpu := (outpu os1)(1 := xs)\<rparr>\<close>
             have step_Tau_1: \<open>step Tau
   (dataflow_op sg (map_op (case_sum id id) (case_sum id id) (comp_op [Inr (0, 1) \<mapsto> Inr (1, 1)] buf
-    (my_ooo_input_op os1) (my_increment_op inc os2))))
+    (my_ooo_input_op os1) (my_incr_op inc os2))))
   (dataflow_op sg (map_op (case_sum id id) (case_sum id id) (comp_op [Inr (0, 1) \<mapsto> Inr (1, 1)] (BENQ (Inr (1, 1)) (Inr (d, t')) buf)
-    (my_ooo_input_op ?os1') (my_increment_op inc os2))))\<close> using that(1) Cons t'(2)
+    (my_ooo_input_op ?os1') (my_incr_op inc os2))))\<close> using that(1) Cons t'(2)
               unfolding invariant_def my_ooo_input_op_def ooo_input_op_def
               by (auto intro!: step_Tau_dataflow_op_Tau_intro)
             let ?os2_1 = \<open>consumes os2 1 t' d\<close>
             have step_Tau_2: \<open>step Tau
   (dataflow_op sg (map_op (case_sum id id) (case_sum id id) (comp_op [Inr (0, 1) \<mapsto> Inr (1, 1)] (BENQ (Inr (1, 1)) (Inr (d, t')) buf)
-    (my_ooo_input_op ?os1') (my_increment_op inc os2))))
+    (my_ooo_input_op ?os1') (my_incr_op inc os2))))
   (dataflow_op sg (map_op (case_sum id id) (case_sum id id) (comp_op [Inr (0, 1) \<mapsto> Inr (1, 1)] buf
-    (my_ooo_input_op ?os1') (my_increment_op inc ?os2_1))))\<close> using that(1) buf_Nil
-              unfolding invariant_def my_increment_op_def increment_op_def
+    (my_ooo_input_op ?os1') (my_incr_op inc ?os2_1))))\<close> using that(1) buf_Nil
+              unfolding invariant_def my_incr_op_def incr_op_def
               by (auto intro!: step_Tau_dataflow_op_Tau_intro)
-            obtain os2_2 where os2_2: \<open>os2_2 |\<in>| increment_op_logic 1 1 inc ?os2_1\<close>
-              unfolding increment_op_logic_def invariant_def trace_simp
+            obtain os2_2 where os2_2: \<open>os2_2 |\<in>| incr_op_logic 1 1 inc ?os2_1\<close>
+              unfolding incr_op_logic_def invariant_def trace_simp
               using SIM2(1) invariant_def by auto
-            hence initia_os2_2: \<open>initia os2_2\<close> using that(1) unfolding invariant_def increment_op_logic_def
+            hence initia_os2_2: \<open>initia os2_2\<close> using that(1) unfolding invariant_def incr_op_logic_def
                 consumes_def add_caps_def drop_caps_def produces_def by simp
-            have input_os2_2: \<open>input os2_2 1 = []\<close> using os2_2 unfolding increment_op_logic_def by (simp split: prod.splits if_splits)
+            have input_os2_2: \<open>input os2_2 1 = []\<close> using os2_2 unfolding incr_op_logic_def by (simp split: prod.splits if_splits)
             have outpu_os2_2: \<open>outpu os2_2 1 = [(d, t)]\<close> using outpu_os2_Nil input_os2_Nil os2_2 t'(1)
-              unfolding increment_op_logic_def consumes_def add_caps_def drop_caps_def produces_def
+              unfolding incr_op_logic_def consumes_def add_caps_def drop_caps_def produces_def
               by (simp split: prod.splits if_splits)
             have summar_os2_2: \<open>intsum os2_2 1 1 = [inc]\<close> using that(1) os2_2 unfolding invariant_def
-                increment_op_logic_def consumes_def add_caps_def drop_caps_def produces_def by simp
-            have ocaps_os2_2: \<open>ocaps os2_2 1 = []\<close> using os2_2 unfolding increment_op_logic_def
+                incr_op_logic_def consumes_def add_caps_def drop_caps_def produces_def by simp
+            have ocaps_os2_2: \<open>ocaps os2_2 1 = []\<close> using os2_2 unfolding incr_op_logic_def
                 consumes_def add_caps_def drop_caps_def produces_def enum_num1_def by (simp add: comp_def split: prod.splits if_splits)
-            have \<open>step Tau (my_increment_op inc ?os2_1) (my_increment_op inc os2_2)\<close> using that(1)
-                Cons os2_2 unfolding invariant_def my_increment_op_def increment_op_def consumes_def
+            have \<open>step Tau (my_incr_op inc ?os2_1) (my_incr_op inc os2_2)\<close> using that(1)
+                Cons os2_2 unfolding invariant_def my_incr_op_def incr_op_def consumes_def
                 add_caps_def by (auto intro!: step_builder_op_Silent
-                  simp add: increment_op_logic_front_initia
+                  simp add: incr_op_logic_front_initia
                   operator_state_front_initia_upd_collapse)
             hence step_Tau_3: \<open>step Tau
   (dataflow_op sg (map_op (case_sum id id) (case_sum id id) (comp_op [Inr (0, 1) \<mapsto> Inr (1, 1)] buf
-    (my_ooo_input_op ?os1') (my_increment_op inc ?os2_1))))
+    (my_ooo_input_op ?os1') (my_incr_op inc ?os2_1))))
   (dataflow_op sg (map_op (case_sum id id) (case_sum id id) (comp_op [Inr (0, 1) \<mapsto> Inr (1, 1)] buf
-    (my_ooo_input_op ?os1') (my_increment_op inc os2_2))))\<close> by auto
+    (my_ooo_input_op ?os1') (my_incr_op inc os2_2))))\<close> by auto
             let ?os2_3 = \<open>os2_2\<lparr>outpu := (outpu os2_2)(1 := [])\<rparr>\<close>
-            have \<open>step (Out (Inr (1, 1)) (Inr (d, t))) (my_increment_op inc os2_2) (my_increment_op inc ?os2_3)\<close>
+            have \<open>step (Out (Inr (1, 1)) (Inr (d, t))) (my_incr_op inc os2_2) (my_incr_op inc ?os2_3)\<close>
               using that outpu_os2_Nil input_os2_Nil Cons t'(1) initia_os2_2 outpu_os2_2
-              unfolding invariant_def my_increment_op_def increment_op_def by auto
+              unfolding invariant_def my_incr_op_def incr_op_def by auto
             hence \<open>step (Out (1, 1) (d, t))
   (dataflow_op sg (map_op (case_sum id id) (case_sum id id) (comp_op [Inr (0, 1) \<mapsto> Inr (1, 1)] buf
-    (my_ooo_input_op ?os1') (my_increment_op inc os2_2))))
+    (my_ooo_input_op ?os1') (my_incr_op inc os2_2))))
   (dataflow_op sg (map_op (case_sum id id) (case_sum id id) (comp_op [Inr (0, 1) \<mapsto> Inr (1, 1)] buf
-    (my_ooo_input_op ?os1') (my_increment_op inc ?os2_3))))\<close> by auto
+    (my_ooo_input_op ?os1') (my_incr_op inc ?os2_3))))\<close> by auto
             hence \<open>wstep (Out (1, 1) (d, t))
   (dataflow_op sg (map_op (case_sum id id) (case_sum id id) (comp_op [Inr (0, 1) \<mapsto> Inr (1, 1)] buf
-    (my_ooo_input_op os1) (my_increment_op inc os2))))
+    (my_ooo_input_op os1) (my_incr_op inc os2))))
   (dataflow_op sg (map_op (case_sum id id) (case_sum id id) (comp_op [Inr (0, 1) \<mapsto> Inr (1, 1)] buf
-    (my_ooo_input_op ?os1') (my_increment_op inc ?os2_3))))\<close> using step_Tau_1 step_Tau_2 step_Tau_3
+    (my_ooo_input_op ?os1') (my_incr_op inc ?os2_3))))\<close> using step_Tau_1 step_Tau_2 step_Tau_3
               by fast
             moreover have \<open>map_op (\<lambda>(p :: 1). (1, 1)) (\<lambda>(p :: 1). (1, 1)) (source_op ((\<lambda>(p :: 1). LCons (d, t) lxs)(1 := lxs)))
   = my_source_op f inc ?os1' buf ?os2_3\<close> using that outpu_os2_Nil input_os2_Nil buf_Nil Cons
@@ -386,48 +386,48 @@ next
           let ?buf' = \<open>BTL (Inr (1, 1)) buf\<close>
           have step_Tau_1: \<open>step Tau
   (dataflow_op sg (map_op (case_sum id id) (case_sum id id) (comp_op [Inr (0, 1) \<mapsto> Inr (1, 1)] buf
-    (my_ooo_input_op os1) (my_increment_op inc os2))))
+    (my_ooo_input_op os1) (my_incr_op inc os2))))
   (dataflow_op sg (map_op (case_sum id id) (case_sum id id) (comp_op [Inr (0, 1) \<mapsto> Inr (1, 1)] ?buf'
-    (my_ooo_input_op os1) (my_increment_op inc ?os2_1))))\<close>  using that(1) Cons t'(2)
-            unfolding invariant_def my_increment_op_def increment_op_def
+    (my_ooo_input_op os1) (my_incr_op inc ?os2_1))))\<close>  using that(1) Cons t'(2)
+            unfolding invariant_def my_incr_op_def incr_op_def
             by (auto intro!: step_Tau_dataflow_op_Tau_intro)
-          obtain os2_2 where os2_2: \<open>os2_2 |\<in>| increment_op_logic 1 1 inc ?os2_1\<close>
-            unfolding increment_op_logic_def invariant_def trace_simp
+          obtain os2_2 where os2_2: \<open>os2_2 |\<in>| incr_op_logic 1 1 inc ?os2_1\<close>
+            unfolding incr_op_logic_def invariant_def trace_simp
             using SIM2(1) invariant_def by auto
-          hence initia_os2_2: \<open>initia os2_2\<close> using that(1) unfolding invariant_def increment_op_logic_def
+          hence initia_os2_2: \<open>initia os2_2\<close> using that(1) unfolding invariant_def incr_op_logic_def
               consumes_def add_caps_def drop_caps_def produces_def by simp
-          have input_os2_2: \<open>input os2_2 1 = []\<close> using os2_2 unfolding increment_op_logic_def by (simp add: comp_def split: prod.splits if_splits)
+          have input_os2_2: \<open>input os2_2 1 = []\<close> using os2_2 unfolding incr_op_logic_def by (simp add: comp_def split: prod.splits if_splits)
           have outpu_os2_2: \<open>outpu os2_2 1 = [(d, t)]\<close> using outpu_os2_Nil input_os2_Nil os2_2 t'(1)
-            unfolding increment_op_logic_def consumes_def add_caps_def drop_caps_def produces_def
+            unfolding incr_op_logic_def consumes_def add_caps_def drop_caps_def produces_def
             by (simp add: comp_def split: prod.splits if_splits)
           have summar_os2_2: \<open>intsum os2_2 1 1 = [inc]\<close> using that(1) os2_2 unfolding invariant_def
-              increment_op_logic_def consumes_def add_caps_def drop_caps_def produces_def by simp
-          have ocaps_os2_2: \<open>ocaps os2_2 1 = []\<close> using os2_2 unfolding increment_op_logic_def
+              incr_op_logic_def consumes_def add_caps_def drop_caps_def produces_def by simp
+          have ocaps_os2_2: \<open>ocaps os2_2 1 = []\<close> using os2_2 unfolding incr_op_logic_def
               consumes_def add_caps_def drop_caps_def produces_def enum_num1_def by (simp add: comp_def split: prod.splits if_splits)
-          have \<open>step Tau (my_increment_op inc ?os2_1) (my_increment_op inc os2_2)\<close> using that(1)
-              Cons os2_2 unfolding invariant_def my_increment_op_def increment_op_def consumes_def
+          have \<open>step Tau (my_incr_op inc ?os2_1) (my_incr_op inc os2_2)\<close> using that(1)
+              Cons os2_2 unfolding invariant_def my_incr_op_def incr_op_def consumes_def
               add_caps_def by (auto intro!: step_builder_op_Silent
-                simp add: increment_op_logic_front_initia
+                simp add: incr_op_logic_front_initia
                 operator_state_front_initia_upd_collapse)
           hence step_Tau_2: \<open>step Tau
   (dataflow_op sg (map_op (case_sum id id) (case_sum id id) (comp_op [Inr (0, 1) \<mapsto> Inr (1, 1)] ?buf'
-    (my_ooo_input_op os1) (my_increment_op inc ?os2_1))))
+    (my_ooo_input_op os1) (my_incr_op inc ?os2_1))))
   (dataflow_op sg (map_op (case_sum id id) (case_sum id id) (comp_op [Inr (0, 1) \<mapsto> Inr (1, 1)] ?buf'
-    (my_ooo_input_op os1) (my_increment_op inc os2_2))))\<close> by auto
+    (my_ooo_input_op os1) (my_incr_op inc os2_2))))\<close> by auto
           let ?os2_3 = \<open>os2_2\<lparr>outpu := (outpu os2_2)(1 := [])\<rparr>\<close>
-          have \<open>step (Out (Inr (1, 1)) (Inr (d, t))) (my_increment_op inc os2_2) (my_increment_op inc ?os2_3)\<close>
+          have \<open>step (Out (Inr (1, 1)) (Inr (d, t))) (my_incr_op inc os2_2) (my_incr_op inc ?os2_3)\<close>
             using that outpu_os2_Nil input_os2_Nil Cons t'(1) initia_os2_2 outpu_os2_2
-            unfolding invariant_def my_increment_op_def increment_op_def by auto
+            unfolding invariant_def my_incr_op_def incr_op_def by auto
           hence \<open>step (Out (1, 1) (d, t))
   (dataflow_op sg (map_op (case_sum id id) (case_sum id id) (comp_op [Inr (0, 1) \<mapsto> Inr (1, 1)] ?buf'
-    (my_ooo_input_op os1) (my_increment_op inc os2_2))))
+    (my_ooo_input_op os1) (my_incr_op inc os2_2))))
   (dataflow_op sg (map_op (case_sum id id) (case_sum id id) (comp_op [Inr (0, 1) \<mapsto> Inr (1, 1)] ?buf'
-    (my_ooo_input_op os1) (my_increment_op inc ?os2_3))))\<close> by auto
+    (my_ooo_input_op os1) (my_incr_op inc ?os2_3))))\<close> by auto
           hence \<open>wstep (Out (1, 1) (d, t))
   (dataflow_op sg (map_op (case_sum id id) (case_sum id id) (comp_op [Inr (0, 1) \<mapsto> Inr (1, 1)] buf
-    (my_ooo_input_op os1) (my_increment_op inc os2))))
+    (my_ooo_input_op os1) (my_incr_op inc os2))))
   (dataflow_op sg (map_op (case_sum id id) (case_sum id id) (comp_op [Inr (0, 1) \<mapsto> Inr (1, 1)] ?buf'
-    (my_ooo_input_op os1) (my_increment_op inc ?os2_3))))\<close> using step_Tau_1 step_Tau_2 by fast
+    (my_ooo_input_op os1) (my_incr_op inc ?os2_3))))\<close> using step_Tau_1 step_Tau_2 by fast
           moreover have \<open>map_op (\<lambda>(p :: 1). (1, 1)) (\<lambda>(p :: 1). (1, 1)) (source_op ((\<lambda>(p :: 1). LCons (d, t) lxs)(1 := lxs)))
   = my_source_op f inc os1 ?buf' ?os2_3\<close> using that outpu_os2_Nil input_os2_Nil Cons input_os2_2
             outpu_os2_2 unfolding invariant_def my_source_op_def BTL_def
@@ -439,38 +439,38 @@ next
         qed
       next
         case (Cons _ xs)
-        obtain os2' where os2': \<open>os2' |\<in>| increment_op_logic 1 1 inc os2\<close>
-          unfolding increment_op_logic_def invariant_def trace_simp Let_def
+        obtain os2' where os2': \<open>os2' |\<in>| incr_op_logic 1 1 inc os2\<close>
+          unfolding incr_op_logic_def invariant_def trace_simp Let_def
           using inv invariant_def local.Cons by force
-        hence initia_os2': \<open>initia os2'\<close> using that(1) unfolding invariant_def increment_op_logic_def
+        hence initia_os2': \<open>initia os2'\<close> using that(1) unfolding invariant_def incr_op_logic_def
             drop_caps_def produces_def by (simp add: comp_def split: prod.splits if_splits)
-        have input_os2': \<open>input os2' 1 = []\<close> using os2' unfolding increment_op_logic_def by (simp add: comp_def split: prod.splits if_splits)
+        have input_os2': \<open>input os2' 1 = []\<close> using os2' unfolding incr_op_logic_def by (simp add: comp_def split: prod.splits if_splits)
         have outpu_os2': \<open>outpu os2' 1 = map (\<lambda>(d, t). (d, t + inc)) (input os2 1)\<close>
-          using outpu_os2_Nil os2' unfolding increment_op_logic_def drop_caps_def produces_def
+          using outpu_os2_Nil os2' unfolding incr_op_logic_def drop_caps_def produces_def
           by (simp add: comp_def split: prod.splits if_splits)
         have summar_os2': \<open>intsum os2' 1 1 = [inc]\<close> using that(1) os2' unfolding invariant_def
-            increment_op_logic_def consumes_def add_caps_def drop_caps_def produces_def by (simp add: comp_def split: prod.splits if_splits)
-        have ocaps_os2': \<open>ocaps os2' 1 = []\<close> using os2' unfolding increment_op_logic_def
+            incr_op_logic_def consumes_def add_caps_def drop_caps_def produces_def by (simp add: comp_def split: prod.splits if_splits)
+        have ocaps_os2': \<open>ocaps os2' 1 = []\<close> using os2' unfolding incr_op_logic_def
             consumes_def add_caps_def drop_caps_def produces_def enum_num1_def by (simp add: comp_def split: prod.splits if_splits)
-        have \<open>step Tau (my_increment_op inc os2) (my_increment_op inc os2')\<close> using that(1) Cons os2'
-          unfolding invariant_def my_increment_op_def increment_op_def
+        have \<open>step Tau (my_incr_op inc os2) (my_incr_op inc os2')\<close> using that(1) Cons os2'
+          unfolding invariant_def my_incr_op_def incr_op_def
           by (auto intro!: step_builder_op_Silent
-              simp add: increment_op_logic_front_initia
+              simp add: incr_op_logic_front_initia
               operator_state_front_initia_upd_collapse)
         hence step_Tau: \<open>step Tau
   (dataflow_op sg (map_op (case_sum id id) (case_sum id id) (comp_op [Inr (0, 1) \<mapsto> Inr (1, 1)] buf
-    (my_ooo_input_op os1) (my_increment_op inc os2))))
+    (my_ooo_input_op os1) (my_incr_op inc os2))))
   (dataflow_op sg (map_op (case_sum id id) (case_sum id id) (comp_op [Inr (0, 1) \<mapsto> Inr (1, 1)] buf
-    (my_ooo_input_op os1) (my_increment_op inc os2'))))\<close> by auto
+    (my_ooo_input_op os1) (my_incr_op inc os2'))))\<close> by auto
         let ?os2'' = \<open>os2'\<lparr>outpu := (outpu os2')(1 := tl (outpu os2' 1))\<rparr>\<close>
-        have \<open>step (Out (Inr (1, 1)) (Inr (d, t))) (my_increment_op inc os2') (my_increment_op inc ?os2'')\<close>
-          using that outpu_os2_Nil Cons initia_os2' outpu_os2' unfolding invariant_def my_increment_op_def
-            increment_op_def by auto
+        have \<open>step (Out (Inr (1, 1)) (Inr (d, t))) (my_incr_op inc os2') (my_incr_op inc ?os2'')\<close>
+          using that outpu_os2_Nil Cons initia_os2' outpu_os2' unfolding invariant_def my_incr_op_def
+            incr_op_def by auto
         hence step_Out: \<open>step (Out (1, 1) (d, t))
   (dataflow_op sg (map_op (case_sum id id) (case_sum id id) (comp_op [Inr (0, 1) \<mapsto> Inr (1, 1)] buf
-    (my_ooo_input_op os1) (my_increment_op inc os2'))))
+    (my_ooo_input_op os1) (my_incr_op inc os2'))))
   (dataflow_op sg (map_op (case_sum id id) (case_sum id id) (comp_op [Inr (0, 1) \<mapsto> Inr (1, 1)] buf
-    (my_ooo_input_op os1) (my_increment_op inc ?os2''))))\<close> by auto
+    (my_ooo_input_op os1) (my_incr_op inc ?os2''))))\<close> by auto
         have \<open>map_op (\<lambda>(p :: 1). (1, 1)) (\<lambda>(p :: 1). (1, 1)) (source_op ((\<lambda>(p :: 1). LCons (d, t) lxs)(1 := lxs)))
   = my_source_op f inc os1 buf ?os2''\<close> using that outpu_os2_Nil Cons input_os2' outpu_os2'
           unfolding invariant_def my_source_op_def
@@ -484,10 +484,10 @@ next
       let ?os2' = \<open>os2\<lparr>outpu := (outpu os2)(1 := xs)\<rparr>\<close>
       have \<open>wstep (Out (1, 1) (d, t))
   (dataflow_op sg (map_op (case_sum id id) (case_sum id id) (comp_op [Inr (0, 1) \<mapsto> Inr (1, 1)] buf
-    (my_ooo_input_op os1) (my_increment_op inc os2))))
+    (my_ooo_input_op os1) (my_incr_op inc os2))))
   (dataflow_op sg (map_op (case_sum id id) (case_sum id id) (comp_op [Inr (0, 1) \<mapsto> Inr (1, 1)] buf
-    (my_ooo_input_op os1) (my_increment_op inc ?os2'))))\<close> using that Cons unfolding invariant_def
-        my_increment_op_def increment_op_def by (auto intro!: step_wstep)
+    (my_ooo_input_op os1) (my_incr_op inc ?os2'))))\<close> using that Cons unfolding invariant_def
+        my_incr_op_def incr_op_def by (auto intro!: step_wstep)
       moreover have \<open>map_op (\<lambda>(p :: 1). (1, 1)) (\<lambda>(p :: 1). (1, 1)) (source_op ((\<lambda>(p :: 1). LCons (d, t) lxs)(1 := lxs)))
   = my_source_op f inc os1 buf ?os2'\<close> using that Cons unfolding invariant_def my_source_op_def
         by (auto intro!: arg_cong[where f=\<open>map_op _ _\<close>] arg_cong[where f=source_op])
